\documentclass[12pt]{article} 
\usepackage[utf8]{inputenc}
\usepackage{geometry}
\geometry{letterpaper}
\usepackage{graphicx} 
\usepackage{parskip}
\usepackage{booktabs}
\usepackage{array} 
\usepackage{paralist} 
\usepackage{verbatim}
\usepackage{subfig}
\usepackage{fancyhdr}
\usepackage{sectsty}

\pagestyle{fancy}
\renewcommand{\headrulewidth}{0pt} 
\lhead{}\chead{}\rhead{}
\lfoot{}\cfoot{\thepage}\rfoot{}

%%% SECTION TITLE APPEARANCE
\allsectionsfont{\sffamily\mdseries\upshape} 

%%% ToC (table of contents) APPEARANCE
\usepackage[nottoc,notlof,notlot]{tocbibind} 
\usepackage[titles,subfigure]{tocloft}
\renewcommand{\cftsecfont}{\rmfamily\mdseries\upshape}
\renewcommand{\cftsecpagefont}{\rmfamily\mdseries\upshape} %

\usepackage{amsmath}
\usepackage{amssymb}
\usepackage{empheq}
\usepackage{xcolor}
\renewcommand{\L}[1]{\mathcal{L}\{#1\}}
\newcommand{\ans}[1]{\boxed{\text{#1}}}
\newcommand{\vecs}[1]{\langle #1\rangle}
\renewcommand{\hat}[1]{\widehat{#1}}
\newcommand{\F}[1]{\mathcal{F}(#1)}
\title{APMA 0360: Homework 3}
\author{Milan Capoor}
\date{17 February 2023}

\begin{document}
\maketitle
\section*{Problem 1}
Verify the following statements:
\[u(x, t) = \frac{1}{\sqrt{4\pi Dt}}e^{-\frac{x^2}{4Dt}}\]
\begin{enumerate}
    \item $u(x, t)$ solves the heat equation $u_t = Du_{xx}$
    
    \color{blue}
    \begin{align*}
        u_t &= \frac{d}{dt} \frac{1}{\sqrt{4\pi Dt}}e^{-\frac{x^2}{4Dt}}\\
        &= -\frac{2\pi D}{(4\pi Dt)^{\frac{3}{2}}}e^{-\frac{x^2}{4Dt}} + \left(\frac{1}{\sqrt{4\pi Dt}}\right) \left(\frac{x^2}{4Dt^2}\right) e^{-\frac{x^2}{4Dt}}\\
        &= -\frac{2\pi D}{(4\pi Dt)^{\frac{3}{2}}}e^{-\frac{x^2}{4Dt}} + \frac{Dx^2}{8\sqrt{\pi}(Dt)^{5/2}}e^{-\frac{x^2}{4Dt}}\\
        &= -\frac{2\pi D}{(4\pi Dt)^{\frac{3}{2}}}e^{-\frac{x^2}{4Dt}} + \frac{Dx^2}{8\sqrt{\pi} (Dt)^{5/2}}e^{-\frac{x^2}{4Dt}}\\
        u_x &= \frac{d}{dx} \frac{1}{\sqrt{4\pi Dt}}e^{-\frac{x^2}{4Dt}} = \left(\frac{1}{\sqrt{4\pi Dt}}\right)\left(\frac{-2x}{4Dt}\right)e^{-\frac{x^2}{4Dt}} \\
        u_{xx} &= \left(\frac{1}{\sqrt{4\pi Dt}}\right)\left(\frac{-2}{4Dt}\right)e^{-\frac{x^2}{4Dt}} + \left(\frac{1}{\sqrt{4\pi Dt}}\right)\left(\frac{-2x}{4Dt}\right)^2 e^{-\frac{x^2}{4Dt}}\\
        &= -\frac{1}{4\sqrt{\pi}(Dt)^{3/2}}e^{-\frac{x^2}{4Dt}} + \frac{x^2}{8\sqrt{\pi}(Dt)^{5/2}}e^{-\frac{x^2}{4Dt}}
    \end{align*}

    \[u_t = Du_{xx}\]
    \[-\frac{2\pi D}{(4\pi Dt)^{\frac{3}{2}}}e^{-\frac{x^2}{4Dt}} + \frac{Dx^2}{8\sqrt{\pi} (Dt)^{5/2}}e^{-\frac{x^2}{4Dt}} = D(-\frac{1}{4\sqrt{\pi}(Dt)^{3/2}}e^{-\frac{x^2}{4Dt}} + \frac{x^2}{8\sqrt{\pi}(Dt)^{5/2}}e^{-\frac{x^2}{4Dt}})\]
    \[-\frac{2\pi D}{(4\pi Dt)^{\frac{3}{2}}} + \frac{Dx^2}{8\sqrt{\pi} (Dt)^{5/2}} = D(-\frac{1}{4\sqrt{\pi}(Dt)^{3/2}} + \frac{x^2}{8\sqrt{\pi}(Dt)^{5/2}})\]
    \[D(-\frac{1}{4\sqrt{\pi}(Dt)^{3/2}} + \frac{x^2}{8\sqrt{\pi} (Dt)^{5/2}}) = D(-\frac{1}{4\sqrt{\pi}(Dt)^{3/2}} + \frac{x^2}{8\sqrt{\pi}(Dt)^{5/2}}) \quad \checkmark\]

    \color{black}
    \item $\int_{-\infty}^\infty u(x, t) \; dx = 1$ for all t 
    
    \color{blue}
    \[\int_{-\infty}^\infty \frac{1}{\sqrt{4\pi Dt}}e^{-\frac{x^2}{4Dt}} \; dx = 1\]
    \[\frac{1}{\sqrt{4\pi Dt}}\int_{-\infty}^\infty e^{-\frac{x^2}{4Dt}} \; dx = 1 \]

    Now let 
    \[I = \int_{-\infty}^\infty e^{-\frac{x^2}{4Dt}} \; dx = \int_{-\infty}^\infty e^{-\frac{x^2}{4Dt}} \; dx \]
    So 
    \begin{align*}
        I^2 &= \left(\int_{-\infty}^\infty e^{-\frac{x^2}{4Dt}} \; dx \right)\left(\int_{-\infty}^\infty e^{-\frac{y^2}{4Dt}} \; dy \right)\\
        &= \int_{0}^\pi \int_{0}^\infty re^{-\frac{r^2}{4Dt}} \; dr \, d\theta\\
        &= 2\pi \int_{0}^\infty re^{-\frac{r^2}{4Dt}} \; dr\\
        u &= -\frac{r^2}{4Dt} \implies du = -\frac{2r}{4Dt}\; dr\\
        I^2 &= 2\pi \left[-2Dt e^{-\frac{r^2}{4Dt}}\right]_0^\infty\\
        &= 2\pi(0 + 2Dt) = 4\pi Dt
    \end{align*}
    Therefore, 
    \[I = \sqrt{4\pi Dt}\]
    and 
    \[\int_{-\infty}^\infty u(x, t) \; dx = \frac{\sqrt{4\pi Dt}}{\sqrt{4\pi Dt}} = 1 \quad \checkmark\]
\end{enumerate}

\pagebreak
\section*{Problem  2}
Consider the Korteweg-De Vries equation
\[\begin{cases}
    u_t = u_{xxx}\\
    u(x, 0) = f(x)
\end{cases}\]
Find a formula for $\hat{u}(\kappa, t)$ in terms of $\hat{f}(\kappa)$

\color{blue}
\[\F{u_t} = \F{u_{xxx}}\]
By the derivative properties of  the fourier transform,
\[\F{u_{xxx}} = (-i\kappa)^3 \hat{u}(\kappa, t) = i\kappa^3 \hat{u}(\kappa, t)\]
and then 
\[\F{u_t} = \frac{d}{dt}\hat{u}(\kappa, t)\]
Thus,
\[\frac{d}{dt}\hat{u}(\kappa, t) =  i\kappa^3 \hat{u}(\kappa, t)\]
Solving by ODE analogy ($y' = ay$),
\[\hat{u}(\kappa, t) = \hat{u}(\kappa, 0)e^{i\kappa^3t}\]
But from the initial condition
\[u(x, 0) = f(x) \longrightarrow \hat{u}(\kappa, 0) = \hat{f}(\kappa)\]
So,
\[\ans{$\hat{u}(\kappa, t) = \hat{f}(\kappa)e^{i\kappa^3t}$}\]


\pagebreak
\color{black}
\section*{Problem 3}
In this problem, a and c are real numbers
\begin{enumerate}
    \color{black}
    \item Show that if $g(x) = f(x - a)$ then $\hat{g}(\kappa) = e^{i\kappa a}\hat{f}(\kappa)$
    
    \color{blue}
    \begin{align*}
        \hat{g}(\kappa) &= \hat{f}(x - a)\\
        &= \int_{-\infty}^\infty f(x - a) e^{i\kappa(x + a)}\; dx\\
        &= e^{i\kappa a}\int_{-\infty}^\infty f(x - a) e^{i\kappa x}\; dx\\
        &= e^{i\kappa a}\hat{f}(\kappa) \quad \checkmark
    \end{align*}
    \color{black}
    \item Use the Fourier transform and (1) to solve the transport PDE
    \[\begin{cases}
        u_t + cu_x = 0\\
        u(x, 0) = f(x)
    \end{cases}\]

    \color{blue}
    \[\hat{u}(\kappa)_t = \F{-cu_x}\]
    \[\frac{d}{dt}\hat{u}(\kappa, t) = i\kappa c\hat{u}(\kappa, t)\]
    \begin{align*}
        \hat{u}(\kappa, t) &= \F{u(x, 0)} e^{i\kappa c}\\
        &= \hat{f}(\kappa)e^{i\kappa ct}\\ 
        &= \hat{f}(x - ct)
    \end{align*}
    \[\boxed{u(x, t) = f(x - ct)}\]
\end{enumerate}

\pagebreak
\section*{Problem 4}
Use the Fourier transform to solve the PDE
\[\begin{cases}
    u_t = Du_{xx} - au\\
    u(x, 0) = f(x)
\end{cases}\]
Here $D > 0$ and a is any real number.\footnote{Write the answer in the form
\[u(x, t) = e^{-at} \times \text{ Some integral}\]}

\color{blue}
\[\hat{u}_t = \F{Du_{xx}} - \F{au}\]
\[\frac{d}{dt}\hat{u}(\kappa, t) = -D\kappa^2\hat{u}(\kappa, t) - a\hat{u}(\kappa, t) = -(D\kappa^2 + a)\hat{u}(\kappa, t)\]
Via ODEs, 
\[\hat{u}(\kappa, t) = \hat{u}(\kappa, 0)e^{-(D\kappa^2 + a)t} = e^{-at} \hat{f}(\kappa) e^{-D\kappa^2t} = \]
Now to set up the convolution:
\[\F{e^{-D\kappa^2t}} = \hat{g}(\kappa, t) \quad g(x, t) = \frac{1}{\sqrt{4\pi Dt}}e^{-\frac{x^2}{4Dt}}\]
Therefore, 
\[\hat{u}(\kappa, t) = e^{-at} \hat{f}(\kappa) \hat{g}(\kappa, t)\]
\[\hat{u}(\kappa, t) = e^{-at}\F{(f \star g)(\kappa, t)}\]
\[\boxed{u(x, t) = \frac{e^{-at}}{\sqrt{4\pi Dt}}\int_{-\infty}^\infty f(y) e^{-\frac{(x-y)^2}{4Dt}}\; dy}\]


\pagebreak 
\color{black}
\section*{Problem 5}
Solve the PDE 
\[\begin{cases}
    u_t = Du_{xx} + cu_x - au\\
    u(x, 0) = f(x)
\end{cases}\]
Here $D > 0$ and a, c are real numbers \footnote{Hint: Let $v(x, t) = u(x - ct, t)e^{at}$ and find a PDE for v}

\color{blue}
Let 
\[v(x, t) = u(x - ct, t)e^{at}\]
so 
\[u(x - ct, t) = v(x, t)e^{at}\]
and 
\[u(x, t) = v(x + ct, t)e^{at}\]
Taking the partials we have:
\[\begin{cases}
    u_x = v_x(x + ct, t)e^{at}\\
    u_{xx} = v_{xx}(x + ct, t)e^{at}\\
    u_t = \frac{\partial v}{\partial x}\frac{\partial x}{\partial t} + \frac{\partial v}{\partial t}\frac{\partial t}{\partial t} = cv_x(x + ct, t)e^{at} + v_t(x + ct, t)e^{at} + av(x + ct, t)e^{at}
\end{cases}\]
and substituting these into the original PDE, 
\[cv_x(x + ct, t)e^{at} + v_t(x + ct, t)e^{at} + av(x + ct, t)e^{at} = Dv_{xx}(x + ct, t)e^{at} + cv_x(x + ct, t)e^{at} - av(x + ct, t)e^{at}\]
But this is just 
\[v_t(x + ct, t) = Dv_{xx}(x + ct, t)\]
And this is simply the heat equation so 
\[v(x + ct, t) = \frac{1}{\sqrt{4\pi Dt}} \int_{-\infty}^\infty f(y)\, e^{-\frac{((x + ct) - y)^2}{4Dt}}\; dy\]
and as 
\[v(x + ct, t) = u(x, t)e^{-at}\]
we have  
\[\boxed{u(x, t) = \frac{e^{at}}{\sqrt{4\pi Dt}} \int_{-\infty}^\infty f(y)\, e^{-\frac{((x + ct) - y)^2}{4Dt}}\; dy}\]
\end{document}
