\documentclass[12pt]{article} 
\usepackage[utf8]{inputenc}
\usepackage{geometry}
\geometry{letterpaper}
\usepackage{graphicx} 
\usepackage{parskip}
\usepackage{booktabs}
\usepackage{array} 
\usepackage{paralist} 
\usepackage{verbatim}
\usepackage{subfig}
\usepackage{fancyhdr}
\usepackage{sectsty}

\pagestyle{fancy}
\renewcommand{\headrulewidth}{0pt} 
\lhead{}\chead{}\rhead{}
\lfoot{}\cfoot{\thepage}\rfoot{}

%%% SECTION TITLE APPEARANCE
\allsectionsfont{\sffamily\mdseries\upshape} 

%%% ToC (table of contents) APPEARANCE
\usepackage[nottoc,notlof,notlot]{tocbibind} 
\usepackage[titles,subfigure]{tocloft}
\renewcommand{\cftsecfont}{\rmfamily\mdseries\upshape}
\renewcommand{\cftsecpagefont}{\rmfamily\mdseries\upshape} %

\usepackage{amsmath}
\usepackage{amssymb}
\usepackage{empheq}

\renewcommand{\L}[1]{\mathcal{L}{#1}}
\newcommand{\ans}[1]{\boxed{\text{#1}}}

\title{Homework 1}
\author{Milan Capoor}
\date{3 February 2023}

\begin{document}
\maketitle
\textbf{Problem 1:} Find the order of each equation and state if it is linear or non-linear. If it's linear, state if it is homogeneous or inhomogeneous. No justification needed
\begin{enumerate}
    \item $u_t - u_{xxt} + uu_x = 0$ - \ans{3rd order, Nonlinear}
    \item $u_x + e^yu_y = 2$ - \ans{1st order, Linear inhomogeneous}
    \item $u_{xx} - 2u_{yyy} = 0$ - \ans{3rd order, Linear homogeneous}
\end{enumerate}

\pagebreak 

\textbf{Problem 2:} Use the definition of linear transformations to show that the following PDE is linear
\[u_x + x^2 u_{yy} = e^{x+y}\]

Solution:
\[L(u) = u_x + x^2 u_{yy}\]
\begin{align*}
    L(u + v) &= (u + v)_x + x^2 (u+ v)_{yy}\\
    &= u_x + v_x + x^2 u_{yy} + x^2 v_{yy}\\
    &= u_x + x^2 u_{yy} + v_x + x^2 v_{yy}\\
    &= L(u) + L(v) \checkmark
\end{align*}

\begin{align*}
    L(cu) &= (cu)_x + x^2 (cu)_{yy}\\
    &= cu_x + cx^2 u_{yy}\\
    &= c(u_x + x^2 u_{yy}) = cL(u) \checkmark
\end{align*}

\pagebreak 

\textbf{Problem 3:} Show that $u(x, y) = f(x) \; g(y)$ solves the PDE 
\[uu_{xy} = u_x u_y\]

Solution:
\[(f(x)g(y))(f(x)g(y))_{xy} = (f(x)g(y))_x (f(x)g(y))_y\]
\[(f(x)g(y))(f'(x)g(y))_y = (f'(x)g(y)(f(x)g(y)))_y\]
\[(f(x)g(y))(f'(x)g'(y)) = (f'(x)g(y))(f(x)g'(y))\]
\[(f(x)g(y))(f'(x)g'(y)) = (f'(x)g'(y))(f(x)g(y)) \checkmark\] 

\pagebreak 

\textbf{Problem 4:} Solve and check 
\[3u_y + u_{xy} = 0\]

Solution:
\[v = u_y \implies 3v + v_x = 0\]

By ODE analogy:
\[v= f(y)e^{-3x}\]
\[u_y = f(y)e^{-3x}\]
\[u = \int f(y) e^{-3x} \; dy = \ans{$F(y) e^{-3x} + G(x)$}\]

Check:
\begin{align*}
    u &= F(y) e^{-3x} + G(x)\\
    u_y &= f(y) e^{-3x}\\
    u_{xy} &= -3f(y) e^{-3x}
    3u_y + u_{xy} = 3f(y) e^{-3x} -3f(y) e^{-3x} = 0 \checkmark
\end{align*}
\pagebreak 

\textbf{Problem 5:} Solve 
\[u_{yy} - 5u_y + 6u = 0\]

By ODE analogy:
\[r^2 - 5r + 6 = 0 \implies (r - 3)(r - 2) = 0 \implies r = \{2, 3\}\]
\[\ans{$u(x, y) = A(x)e^{2y} + B(x)e^{3y}$}\]

\pagebreak 

\textbf{Problem 6:} What is the type of the following 2nd order PDE:
\begin{enumerate}
    \item $u_{xx} - 4u_{xy} + u_{yy} + 2u_y + 4u = 0$
    \[D = (-4)^2 - 4(1)(1) = 12 > 0 \implies \ans{ Hyperbolic}\]
    \item $9u_{xx} + 6u_{xt} + u_{tt} + u_x = x^2$
    \[D = (-6)^2 + 4(9)(1) = 0 \implies \ans{ parabolic}\]
\end{enumerate}

\pagebreak 

\textbf{Problem 7:} Find all real numbers $\alpha$ such that 
\[u(x, y, z) = (x^2 + y^2 + z^2)^\alpha\]
is a solution of $u_{xx} + u_{yy} + u_{zz} = 0$

Solution:
\begin{align*}
    u_x &= 2x\alpha(x^2 + y^2 + z^2)^{\alpha - 1}\\
    u_y &= 2y\alpha(x^2 + y^2 + z^2)^{\alpha - 1}\\
    u_z &= 2z\alpha(x^2 + y^2 + z^2)^{\alpha - 1}
\end{align*}
\begin{align*}
    u_{xx} &= 2\alpha(x^2 + y^2 + z^2)^{\alpha - 1} + 4x^2\alpha(\alpha - 1)(x^2 + y^2 + z^2)^{\alpha - 2}\\
    u_{yy} &= 2\alpha(x^2 + y^2 + z^2)^{\alpha - 1} + 4y^2\alpha(\alpha - 1)(x^2 + y^2 + z^2)^{\alpha - 2}\\
    u_{zz} &= 2\alpha(x^2 + y^2 + z^2)^{\alpha - 1} + 4z^2\alpha(\alpha - 1)(x^2 + y^2 + z^2)^{\alpha - 2}\\
\end{align*}
\begin{align*}
    0 &= u_{xx} + u_{yy} + u_{zz} \\
    &= 6\alpha(x^2 + y^2 + z^2)^{\alpha - 1} + 4\alpha(\alpha - 1)(x^2 + y^2 + z^2)^{\alpha - 2}(x^2 + y^2 + z^2)\\
    &= 6\alpha(x^2 + y^2 + z^2)^{\alpha - 1} + 4\alpha(\alpha - 1)(x^2 + y^2 + z^2)^{\alpha - 1}\\
    &= (6\alpha + 4\alpha^2 - 4\alpha)(x^2 + y^2 + z^2)^{\alpha - 1}\\
    &= (2\alpha)(1 + 2\alpha)(x^2 + y^2 + z^2)^{\alpha - 1}\\
\end{align*}

The above equation is undefined for $\alpha <= 0 \cap (x, y, z) = (0, 0, 0)$ and positive for all other values. Thus, the only real numbers for which $u(x, y, z) = (x^2 + y^2 + z^2)^\alpha$ satisfies $u_{xx} + u_{yy} + u_{zz} = 0$ are

\begin{center}
    \ans{$\alpha = \{0, -\frac{1}{2}\}$ given that $(x, y, z) \neq (0, 0, 0)$ and $\alpha = -\frac{1}{2}$ otherwise}
\end{center}

\end{document}
